add compare and swap model

fstar/MemoryModel.fst
@@ -12,10 +12,29 @@ noeq type state_t = {
      bytemap: Map.t U16.t U8.t;
   }
 
+
+
 assume val r0: P.preorder state_t
 assume val r1: P.preorder state_t
 
 let state_prop = state_t -> prop
+
+// pre-condition for write the value `v` at the index `k`
+let write_pre0 (k:U16.t) (v:U8.t) (p0:state_prop) : prop =
+  forall s. p0 s ==> r0 s {bytemap = Map.upd s.bytemap k v}
+
+let write_post0 (k:U16.t) (v:U8.t) (p0:state_prop) (p1:state_prop) : prop =
+  forall y. p1 y <==> (exists x.
+    p0 x /\ r1 {bytemap = Map.upd x.bytemap k v} y
+  )
+
+let read_post0 (k:U16.t) (p0:state_prop) (v:U8.t) (p1:state_prop) : prop =
+  let p (s:state_t) =
+    p0 s /\ Map.sel s.bytemap k == v
+  in (exists s. p s) /\ (forall y. p1 y <==> (
+    exists x. p x /\ r1 x y
+  ))
+
 new_effect NONDET_STATE = STATE_h state_prop
 
 unfold let lift_div_state (a:Type) (wp:pure_wp a) (p:a -> state_prop -> Type0) (h:state_prop) =
@@ -31,22 +50,25 @@ effect ST (a:Type)
 
 effect St (a:Type) = ST a (fun h -> True) (fun h0 r h1 -> True)
 
-assume val read0 (x:U16.t) :
+assume val read0 (k:U16.t) :
   ST U8.t
     (fun p0 -> True)
-    (fun p0 v p1 -> 
-      let p (s:state_t) : prop = 
-        p0 s /\ Map.sel s.bytemap x == v
-      in
-      (exists s. p s) /\ (forall y. p1 y <==> (
-        exists x. r1 x y /\ p x
+    (read_post0 k)
+
+assume val write0 (k:U16.t) (v:U8.t) :
+  ST unit
+    (write_pre0 k v)
+    (fun p0 _ -> write_post0 k v p0)
+
+
+assume val cas0 (key:U16.t) (old_v new_v:U8.t) :
+  ST (option U8.t)
+    (fun p0 -> True)
+    (fun p0 r p1 ->
+      (None? r ==>
+        write_pre0 key new_v (fun s -> p0 s /\ Map.sel s.bytemap key == old_v) /\
+        write_post0 key new_v (fun s -> p0 s /\ Map.sel s.bytemap key == old_v) p1
+      ) /\ (Some? r ==> (r <> Some old_v /\
+        read_post0 key p0 (match r with | Some x -> x) p1
       ))
     )
-
-assume val write0 (key:U16.t) (v:U8.t) :
-  ST unit
-    (fun p0 -> forall s. p0 s ==> r1 s {bytemap = Map.upd s.bytemap key v})
-    (fun p0 _ p1 -> forall y. p1 y <==> (
-      exists x. p0 x /\ r1 {bytemap = Map.upd x.bytemap key v} y
-    ))
-
